Removed attributesInQuery

RelationalAlgebra/FOL/Schema.lean
@@ -4,6 +4,7 @@ open FOL FirstOrder Language RM Term
 
 namespace FOL
 
+-- Extend ModelTheory
 @[simp]
 theorem BoundedFormula.exs.freeVarFinset {k} (φ : fol.BoundedFormula Attribute k) :
   (φ.exs).freeVarFinset = φ.freeVarFinset := by
@@ -12,60 +13,27 @@ theorem BoundedFormula.exs.freeVarFinset {k} (φ : fol.BoundedFormula Attribute 
     . simp [BoundedFormula.exs]
       simp_all only [BoundedFormula.freeVarFinset, Finset.union_empty]
 
--- Attributes in query
-def BoundedQuery.attributesInQuery {n : ℕ} (q : BoundedQuery n) : Finset Attribute := q.toFormula.freeVarFinset
-
-@[simp]
-theorem BoundedQuery.attributesInQuery.R_def_mem [folStruc] {n : ℕ} {x : Attribute} (t : Fin (dbs rn).card → fol.Term (Attribute ⊕ Fin n)) :
-  x ∈ (R dbs rn t).attributesInQuery ↔ ∃i : Fin (dbs rn).card, x ∈ (t i).varFinsetLeft := by
-    simp_all only [attributesInQuery, toFormula, Relations.boundedFormula,
-      BoundedFormula.freeVarFinset, Finset.mem_biUnion, Finset.mem_univ, true_and]
-
-instance BoundedQuery.attributesInQuery.R_fintype [folStruc] {rn} {dbs : DatabaseSchema} {t : Fin (dbs rn).card → fol.Term (Attribute ⊕ Fin n)} :
-  Fintype {a | ∃i : Fin (dbs rn).card, a ∈ (t i).varFinsetLeft} := by
-    apply Fintype.ofFinset ((BoundedQuery.R dbs rn t).attributesInQuery)
-    simp_all [BoundedQuery.attributesInQuery.R_def_mem]
-
-@[simp]
-theorem BoundedQuery.attributesInQuery.R_def [folStruc] {n : ℕ} (t : Fin (dbs rn).card → fol.Term (Attribute ⊕ Fin n)) :
-  (R dbs rn t).attributesInQuery = {a | ∃i : Fin (dbs rn).card, a ∈ (t i).varFinsetLeft}.toFinset := by
-    exact Eq.symm (Set.toFinset_ofFinset (R dbs rn t).attributesInQuery R_fintype._proof_2)
-
-@[simp]
-theorem BoundedQuery.attributesInQuery.tEq_def {n : ℕ} (q : BoundedQuery n) (t₁ t₂ : fol.Term (Attribute ⊕ Fin n)) :
-  (tEq q t₁ t₂).attributesInQuery = q.attributesInQuery ∪ t₁.varFinsetLeft ∪ t₂.varFinsetLeft := by simp_all [attributesInQuery, toFormula]
-
-@[simp]
-theorem BoundedQuery.attributesInQuery.and_def {n : ℕ} (q₁ q₂ : BoundedQuery n) :
-  (and q₁ q₂).attributesInQuery = q₁.attributesInQuery ∪ q₂.attributesInQuery := by simp_all [attributesInQuery, toFormula]
-
-@[simp]
-theorem BoundedQuery.attributesInQuery.ex_def {n : ℕ} (q : BoundedQuery (n + 1)) :
-  (ex q).attributesInQuery = q.attributesInQuery := by simp_all [attributesInQuery, toFormula]
-
-@[simp]
-theorem BoundedQuery.attributesInQuery.exs_def {n : ℕ} (q : BoundedQuery n) :
-  (exs q).attributesInQuery = q.attributesInQuery := by simp [attributesInQuery]
-
-
 -- schema of query
 def BoundedQuery.schema {n : ℕ} : (q : BoundedQuery n) → Finset Attribute
-  | .R dbs name vMap => (R dbs name vMap).attributesInQuery
+  | .R dbs name vMap => (R dbs name vMap).toFormula.freeVarFinset
   | .tEq q _ _ => q.schema
   | .and q1 q2 => q1.schema ∪ q2.schema
   | .ex q => q.schema
 
-theorem BoundedQuery.schema.sub_attributesInQuery {n} (q : BoundedQuery n) : q.schema ⊆ q.attributesInQuery := by
-  induction q
-  all_goals simp_all [BoundedQuery.schema, attributesInQuery, BoundedQuery.toFormula, Finset.union_subset_union]
-  . rw [Finset.subset_iff]; aesop
+@[simp]
+theorem BoundedQuery.schema.R_def_mem [folStruc] {n : ℕ} {x : Attribute} (t : Fin (dbs rn).card → fol.Term (Attribute ⊕ Fin n)) :
+  x ∈ (R dbs rn t).schema ↔ ∃i : Fin (dbs rn).card, x ∈ (t i).varFinsetLeft := by
+    simp_all only [schema, toFormula, Relations.boundedFormula,
+      BoundedFormula.freeVarFinset, Finset.mem_biUnion, Finset.mem_univ, true_and]
 
-theorem BoundedQuery.schema.sub_attributesInQuery_mem {x n} (q : BoundedQuery n) : x ∈ q.schema → x ∈ q.attributesInQuery :=
-  fun a ↦ BoundedQuery.schema.sub_attributesInQuery q a
+instance BoundedQuery.schema.R_fintype [folStruc] {rn} {dbs : DatabaseSchema} {t : Fin (dbs rn).card → fol.Term (Attribute ⊕ Fin n)} :
+  Fintype {a | ∃i : Fin (dbs rn).card, a ∈ (t i).varFinsetLeft} := by
+    apply Fintype.ofFinset ((BoundedQuery.R dbs rn t).schema)
+    simp only [BoundedQuery.schema.R_def_mem, Set.mem_setOf_eq, implies_true]
 
 @[simp]
 theorem BoundedQuery.schema.R_def [folStruc] {n : ℕ} (t : Fin (dbs rn).card → fol.Term (Attribute ⊕ Fin n)) :
-  (R dbs rn t).schema = (R dbs rn t).attributesInQuery := by rfl
+  (R dbs rn t).schema = {a | ∃i : Fin (dbs rn).card, a ∈ (t i).varFinsetLeft}.toFinset := by ext a; simp
 
 @[simp]
 theorem BoundedQuery.schema.tEq_def {n : ℕ} (q : BoundedQuery n) (t₁ t₂ : fol.Term (Attribute ⊕ Fin n)) :
